Copypasta from SeqNumCorrect

systems/DiskCorrect.v
@@ -18,12 +18,55 @@ Section DiskCorrect.
     @mkPacket _ orig_multi_params (d_pSrc p) (d_pDst p) (d_pBody p).
 
   Definition revertDiskNetwork (net: disk_network) : orig_network :=
-    mkNetwork (map revertPacket (nwdPackets net)) (fun h => nwdState net h).
+    mkNetwork (map revertPacket (nwdPackets net)) (nwdState net).
+  
+  Lemma reachable_revert_step :
+    forall st st' out,
+      reachable step_async_disk step_async_disk_init st ->
+      step_async_disk st st' out ->
+      (exists out, step_async (revertDiskNetwork st) (revertDiskNetwork st') out).
+  Proof using.
+    intros.
+    unfold reachable in *.
+    break_exists.
+    match goal with H : step_async_disk _ _ _ |- _ => invcs H end.
+    - admit.
+    - admit.
+  Admitted.
+  
+  Theorem reachable_revert :
+    true_in_reachable step_async_disk step_async_disk_init
+                      (fun (st : disk_network) =>
+                         reachable step_async
+                                   step_async_init
+                                   (revertDiskNetwork st)).
+  Proof.
+    apply true_in_reachable_reqs.
+    - unfold revertDiskNetwork. simpl.
+      unfold reachable. exists []. constructor.
+    - intros.
+      find_apply_lem_hyp reachable_revert_step; auto.
+      intuition.
+      unfold reachable in *.
+      break_exists.
+      eexists.
+      apply refl_trans_n1_1n_trace.
+      econstructor;
+        eauto using refl_trans_1n_n1_trace.
+  Qed.
 
   Theorem true_in_reachable_disk_transform :
     forall P,
       true_in_reachable step_async step_async_init P ->
       true_in_reachable step_async_disk step_async_disk_init (fun net => P (revertDiskNetwork net)).
   Proof.
-  Admitted.
+    intros.
+    intros. find_apply_lem_hyp true_in_reachable_elim. intuition.
+    apply true_in_reachable_reqs; eauto.
+    intros. find_copy_apply_lem_hyp reachable_revert.
+    find_apply_lem_hyp reachable_revert_step; auto.
+    intuition.
+    break_exists.
+    eauto.
+  Qed.
 End DiskCorrect.
